updated Breadboard for variadic arguments

BreadBoard/Breadboard.v
@@ -2,13 +2,28 @@
 Require Import List.
 Require Import ListSet.
 Require Import EqNat.
+Import ListNotations.
 
 Require Import Arith.
-   Open Scope list_scope.
+Open Scope list_scope.
 Module Type IO_SIG.
   Variable t : Type.
+  Variable trace : Set.
   Variable func : Set.
+  Variable nargs : func -> nat.
 End IO_SIG.
+
+Module IO.
+  Definition t :=  nat.
+  Definition trace := list (list t).
+  Inductive func_ :=
+  | fn_args : nat -> (trace -> t) -> func_.
+  Definition func := func_.
+  Definition nargs f :=
+    match f with
+      | fn_args n _ => n
+    end.
+End IO.
 
 Module Type Component_Sig(IO:IO_SIG).
   Variable io : IO.func.
@@ -20,42 +35,94 @@ Module Component(I:IO_SIG)(M:Component_Sig(I)).
 End Component.
 
 Module Wiring(IO:IO_SIG).
-Inductive wiring :=
+  Inductive wiring :=
   | base :  wiring
-  | watch_set :  wiring -> nat -> IO.func -> nat ->  wiring
-  | just_set : wiring  -> IO.func -> nat -> wiring.
-Notation  "w //  m ~> f ~>  n" := (watch_set w m f n) (at level 80, m at next level). 
-Notation  "w */  f ~>  n" := (just_set w f n) (at level 80, m at next level). 
+  | watch_set :  wiring -> list nat -> IO.func -> nat ->  wiring
+  | just_set : wiring  -> IO.func -> nat -> wiring
+  | join : wiring -> wiring -> wiring.
+  Notation  "w //  m ~> f ~>  n" := (watch_set w m f n) (at level 80, m at next level). 
+  Notation  "w */  f ~>  n" := (just_set w f n) (at level 80, m at next level). 
+
+  Notation "w1 ~&~ w2" := (join w1 w2) (at level 80).
 
 
-(* Checks that all observers have a source and that only one setter per nat *)
-Fixpoint valid_wiring' w ins outs: Prop :=
-  let add_i := set_add%nat nat eq_nat_dec in
-  let notin := (fun el  s => (not (set_In%nat nat  el s))) in
-  match w with 
-    | base  =>
-      (set_inter%nat nat eq_nat_dec ins outs) = ins
-    | watch_set w' from fn to =>
-      notin to outs /\  valid_wiring' w' ( add_i from ins) (add_i to outs)
-    | just_set w' fn to=>
-      notin to outs /\ valid_wiring' w' ins (add_i to outs)
-  end.
-Definition valid_wiring w : Prop :=
-  valid_wiring' w nil nil.
+  Fixpoint output_pins w s: set nat :=
+    let add_i := set_add%nat nat eq_nat_dec in
+    match w with 
+      | base  =>
+        s
+      | watch_set w' from fn to =>
+        output_pins w' (add_i  to s)
+      | just_set w' fn to =>
+        output_pins w' (add_i to s)
+      | join w1 w2 => set_union%nat nat eq_nat_dec (output_pins w1 s) (output_pins w2 nil)
+    end.
 
-Require Import Omega.
-Ltac autowire :=
+  Fixpoint input_pins w s: set nat :=
+    let add_i := set_add%nat nat eq_nat_dec in
+    match w with 
+      | base  => s
+      | watch_set w' from fn to =>
+        output_pins w'
+                    (fold_left (fun se f => add_i f se) s  from)
+
+      | just_set w' fn to =>  output_pins w' s
+      | join w1 w2 => set_union%nat nat eq_nat_dec (output_pins w1 s) (output_pins w2 nil)
+    end.
+
+  Fixpoint all_pins' w s: set nat :=
+    let add_i := set_add%nat nat eq_nat_dec in
+    match w with 
+      | base  => s
+      | watch_set w' from fn to =>
+        all_pins' w'
+                  (add_i to (fold_left (fun se f => add_i f se) s  from))
+
+      | just_set w' fn to =>  all_pins' w' (add_i to s)
+      | join w1 w2 => set_union%nat nat eq_nat_dec (all_pins' w1 s) (all_pins' w2 nil)
+    end.
+  Definition pins w := all_pins' w nil.
+  (* Checks that all observers have a source and that only one setter per nat *)
+  Fixpoint valid_wiring' w ins outs: Prop :=
+    let add_i := set_add%nat nat eq_nat_dec in
+    let notin := (fun el  s => (not (set_In%nat nat  el s))) in
+    let union := set_union%nat nat eq_nat_dec in
+    let intersect := set_inter%nat nat eq_nat_dec in
+    match w with 
+      | base  =>
+        (* Check that the intersection of inputs and outputs is inputs,
+         ie, everything can be read *)
+        (intersect ins outs) = ins
+      | watch_set w' from fn to =>
+        notin to outs /\
+        IO.nargs fn = length from /\
+        valid_wiring' w'
+                      ( fold_left  (fun s f => add_i f s) ins from) (add_i to outs)
+      | just_set w' fn to=>
+        notin to outs
+        /\ valid_wiring' w' ins (add_i to outs)
+      | join w1 w2 =>
+        let w1_out := output_pins w1 [] in
+        let w2_out := output_pins w2 [] in
+        (* intersect w1_out w2_out = [] /\ (*is implicitly checked*)  *) 
+        (* We union in the others outputs to say that w2 is promising
+        that it will make this available as an output (so treat it as an
+        available input too *)
+        valid_wiring' w1 (union w2_out ins) (union
+                                               w2_out outs) /\
+        valid_wiring' w2  (union w1_out ins) (union w1_out outs)
+    end.
+  Definition valid_wiring w : Prop :=
+    valid_wiring' w nil nil.
+
+  Require Import Omega.
+  Ltac autowire :=
     unfold valid_wiring;
     unfold valid_wiring';
-    unfold not;unfold set_add, set_In, set_inter, In;simpl;
+    simpl;
     repeat (try split; try omega).
-
 End Wiring.
 
-Module IO.
-  Definition t := nat.
-  Definition func := list t -> t.
-End IO.
 
 Fixpoint len {T:Type}(x : list T) : nat :=
   match x with
@@ -71,17 +138,8 @@ Fixpoint suml (x : list nat) : nat :=
 Module Wires := Wiring(IO).
 Import Wires.
 
-
 Module IORUN.
 
-  Fixpoint pins' w s: set nat :=
-    let add_i := set_add%nat nat eq_nat_dec in
-    match w with 
-      | base  => s
-      | watch_set w' from fn to => pins' w' (add_i from (add_i to s))
-      | just_set w' fn to =>  pins' w' (add_i to s)
-    end.
-  Definition pins w := pins' w nil.
 
   Definition pin_trace_gen w : list (nat* list IO.t):= map (fun p => (p, nil)) (pins w).
 
@@ -90,6 +148,8 @@ Module IORUN.
       | nil => nil
       | (p', t)::rest => if beq_nat p' p then t else find_trace p rest
     end.
+  Definition find_traces (p :list nat) (pt : list (nat * list IO.t)) : list (list IO.t) :=
+    map (fun f =>  (find_trace f pt))  p.
 
   Definition any_trace  (pt : list (nat * list IO.t) ): list IO.t :=
     match pt with 
@@ -102,23 +162,27 @@ Module IORUN.
         update_trace pt rest ((p, iot::(find_trace p pt))::acc)
       | nil => acc
     end.
+  Print IO.func.
   Fixpoint step' w pt (u : list (nat * IO.t))  :=
     let add_i := set_add in 
     match w with 
       | base  =>
         update_trace pt (u) nil
-      | watch_set w' from fn to =>
-        step' w' pt ((to, fn (find_trace from pt ))::u)
-      |  just_set w' fn to =>
-         step' w' pt  ((to, fn (any_trace  pt ))::u)
+      | watch_set w' from (IO.fn_args n fn) to =>
+        let traces := (find_traces from pt) in
+        step' w' pt ((to, fn traces )::u)
+      |  just_set w' (IO.fn_args n fn) to =>
+         step' w' pt  ((to, fn [any_trace  pt ])::u)
+      | join w1 w2 =>
+        step' w2 pt [] ++ step' w1 pt u
     end.
   Definition step w :=
-    step' w (pin_trace_gen w) nil.
+    step' w (pin_trace_gen w) [].
 
   Fixpoint run' (w:wiring) (pt: list (nat * list IO.t)) fuel  :=
     match fuel with
       | O => pt
-      | S n => run' w (step' w pt nil) n
+      | S n => run' w (step' w pt []) n
     end.
   Definition run w fuel :=
     run' w (pin_trace_gen w) fuel.
@@ -131,65 +195,80 @@ End IORUN.
 
 Import IORUN.
 
-Module Integrator_Spec.
-  Definition io (x:list IO.t):IO.t := suml x.
-End Integrator_Spec.
-Module Incrementor_Spec.
-  Definition io (x:list IO.t):IO.t := len x.
-End Incrementor_Spec.
+(* Module Integrator_Spec. *)
+(*   Definition io (x:list IO.t):IO.t := suml x. *)
+(* End Integrator_Spec. *)
+(* Module Incrementor_Spec. *)
+(*   Definition io (x:list IO.t):IO.t := len x. *)
+(* End Incrementor_Spec. *)
 
 
-  Fixpoint alt x start:=
-    match x with
-      | O => start
-      | S n => alt n (if beq_nat start 0 then 1 else 0)
-    end.
-Module Alternator_Spec.
-  Require Import Arith.Even.
-  Definition io (x:list IO.t):IO.t := alt (length x) 1.
-End Alternator_Spec.
+Fixpoint alt x start:=
+  match x with
+    | O => start
+    | S n => alt n (if beq_nat start 0 then 1 else 0)
+  end.
+(* Module Alternator_Spec. *)
+(*   Require Import Arith.Even. *)
+(*   Definition io (x:list IO.t):IO.t := alt (length x) 1. *)
+(* End Alternator_Spec. *)
 
-Module Integrator := Component(IO)(Integrator_Spec).
-Module Incrementor := Component(IO)(Incrementor_Spec).
-Module Alternator := Component(IO)(Alternator_Spec).
+(* Module Integrator := Component(IO)(Integrator_Spec). *)
+(* Module Incrementor := Component(IO)(Incrementor_Spec). *)
+(* Module Alternator := Component(IO)(Alternator_Spec). *)
 
 
-Definition integrator(x:list IO.t):IO.t := suml x.
-Definition incrementor (x:list IO.t):IO.t := len x.
-Definition alternator (x:list IO.t):IO.t := alt (length x) 1.
-Definition zero_rail (x:list IO.t):IO.t := 0.
+Definition integrator  : IO.func := IO.fn_args 1 (fun x =>suml (hd [] x)).
+Definition incrementor :IO.func := IO.fn_args 1
+                                              (fun x =>len (hd [] x)).
+Definition alternator : IO.func :=IO.fn_args 1
+                                             (fun x =>
+                                                alt (length (hd [] x)) 1).
+Definition zero_rail   : IO.func := IO.fn_args 0 (fun _ =>0).
+
+Definition delay_n n default : IO.func := IO.fn_args 1
+                                                   (fun x => nth n (hd [] x) default).
 
 
 Definition demo1 := base
-                       */  zero_rail ~> 0
-                      //  5 ~> integrator~> 6
-                      // 2 ~> integrator~> 3
-                      */ incrementor~> 2
-                      */ (fun _=> 10) ~> 5
+                      */  zero_rail ~> 0
+                      //  [5] ~> integrator~> 6
+                      // [2] ~> integrator~> 3
+                      */ incrementor ~> 2
+                      */ IO.fn_args 0 (fun _=> 10) ~> 5
                       */ alternator ~> 8.
 
-Theorem good_build : valid_wiring demo1.
+Definition demo2 := base */integrator ~> 9
+// [6] ~> delay_n 5 0 ~> 10.
+
+Theorem good_build : valid_wiring (demo1 ~&~ demo2).
 Proof. 
   autowire.
 Qed.
-Compute (find_trace 3 (run demo1 10)).
+
+Theorem bad_build : valid_wiring (demo1 ~&~ demo1) -> False.
+Proof. 
+  autowire.
+Qed.
+
+Compute (find_trace 10 (run (demo1 ~&~ demo2) 10)).
 
 Theorem alternates: forall n,
-                              let tr := run demo1 n in
-                              let a :=find_trace 8 tr in
-                              n >2 -> (hd 0 a) <> (hd 0 (tl a)).
+                      let tr := run demo1 n in
+                      let a :=find_trace 8 tr in
+                      n >2 -> (hd 0 a) <> (hd 0 (tl a)).
 Proof.
-intros.
+  intros.
 
-intros.
-induction n.
-inversion H.
+  intros.
+  induction n.
+  inversion H.
 
-unfold run, run', step', update_trace, demo1 , alternator, integrator, zero_rail,
-incrementor, find_trace , update_trace, pin_trace_gen, pins, pins', length, alt,
-set_add, set_remove, set_inter in tr.
-simpl in tr.
+  unfold run, run', step', update_trace, demo1 , alternator, integrator, zero_rail,
+  incrementor, find_trace , update_trace, pin_trace_gen, pins, output_pins, length, alt,
+  set_add, set_remove, set_inter in tr.
+  simpl in tr.
 
-unfold a.
-admit. (** :( **)
+  unfold a.
+  admit. (** :( **)
 Qed.
